partial/Memory.v
@@ -1,29 +1,310 @@
+(* Abstract specification of memory *)
+
+
+Inductive lta T n (r : T) : T -> Prop :=
+| lea_self : lta T n r (n r)
+| lea_next r' : lta T n r r' -> lta T n r (n r').
+
+
 Module Type Memory.
 
 Parameter adr : Set.
 
-Parameter first : adr.
+Parameter adr0 : adr.
 Parameter next : adr -> adr.
 
+Parameter dec_eq : forall (r r' : adr),  {r  = r'} + { r <> r'}.
 
+Hint Constructors lta.
 
-Parameter Mem : Type.
+Infix "<" := (lta adr next).
 
-Parameter empty : Mem.
-Parameter get : adr -> Mem -> nat.
-Parameter set : adr -> nat -> Mem -> Mem.
-Parameter free : adr -> Mem -> Mem.
-Parameter freeFrom : adr -> Mem -> Prop.
+Axiom next_fresh : forall (r r' : adr), r < r' -> r <> r'.
 
-Axiom freeFrom_free : forall (r : adr) (m : Mem) (n : nat), freeFrom r m -> free r (set r n m) = m.
+Parameter Mem : Type -> Type.
 
-Axiom freeFrom_set : forall (r : adr) (m : Mem) (n : nat), freeFrom r m  ->  freeFrom (next r) (set r n m).
+Parameter get : forall {T}, adr -> Mem T -> option T.
+Parameter set : forall {T}, adr -> T -> Mem T -> Mem T.
 
-Axiom get_set : forall (r : adr) (m : Mem) (n : nat), get r (set r n m) = n.
-
-Axiom freeFrom_first : freeFrom first empty.
-
-
-
+Axiom get_set : forall T (r : adr) (v : T) (s :  Mem T),
+    get r (set r v s) = Some v.
+Axiom get_get : forall T (r r' : adr) (v : T) (s :  Mem T),
+    r <> r' -> get r (set r' v s) = get r s.
+Axiom set_set : forall T (r : adr) (v v' : T) (s :  Mem T),
+    set r v (set r v' s) = set r v s.
+Axiom set_get : forall T (r : adr) (v : T) (s :  Mem T),
+    get r s = Some v -> set r v  s = s.
 
 End Memory.
+
+Require Import Setoid.  
+Module MemoryTheory (mem : Memory).
+
+Import mem.
+
+
+Definition dom {T} (s : Mem T) (r : adr) : Prop
+  := exists v, get r s = Some v.
+
+
+Notation "x ∈ y" := (@dom _ y x) (at level 70).
+Notation "x ∉ y" := (~(x ∈ y)) (at level 70).
+
+Definition memle {T} (s t : Mem T) : Prop :=
+  forall r, r ∈ s -> get r s = get r t.
+
+
+Infix "=<" := memle  (at level 50).
+
+Lemma not_memle T r (s : Mem T) : r ∉ s -> get r s = None.
+Proof.
+  intros.
+  remember (get r s) as G. destruct G.
+  - assert (exists t, get r s = Some t) as E by eauto. contradiction.
+  - reflexivity.
+Qed.
+
+Lemma memle_set T r v (s : Mem T) : (r ∉ s) ->  s =< set r v s.
+Proof.
+  intros rs r' rs'.
+  remember (dec_eq r r') as R. destruct R.
+  - subst. contradiction.
+  - symmetry. apply get_get. auto.
+Qed.
+
+Lemma memle_get T r v (s t : Mem T) :
+  s =< t -> get r s = Some v -> get r t = Some v.
+Proof.
+  intros. assert (exists t, get r s = Some t) as E by eauto.
+  apply H in E. rewrite <- E. assumption.
+Qed.
+
+Lemma set_dom T r r' v (s : Mem T) : r ∈ s -> r ∈ (set r' v s).
+Proof.
+  intro D. destruct (dec_eq r r').
+  - subst. eexists. rewrite get_set. eauto.
+  - destruct D. eexists. rewrite get_get by eauto. eauto.
+Qed.
+  
+Lemma set_dom_fresh T r r' v (s : Mem T) : r <> r' -> r ∈ (set r' v s) -> r ∈ s.
+Proof.
+  intros I D. destruct D. eexists. rewrite get_get in H by auto. eassumption.
+Qed.
+  
+
+
+Lemma set_monotone T r v (s t : Mem T) :
+  s =< t -> set r v s =< set r v t.
+Proof.
+  intros L r' D. destruct (dec_eq r r').
+  - subst. do 2 rewrite get_set. reflexivity.
+  - do 2 rewrite get_get by auto. apply L. eapply set_dom_fresh; eauto.
+Qed.
+
+  
+Lemma lta_trans (r1 r2 r3 : adr) : r1 < r2 -> r2 < r3 -> r1 < r3.
+Proof.
+  intros R1 R2. induction R2;auto.
+Qed.
+
+Hint Resolve lta_trans.
+
+Definition lea r r' := r < r' \/ r = r'.
+
+Infix "<=" := lea.
+
+
+Fixpoint nextN (n : nat) (r : adr) : adr :=
+  match n with
+  | 0 => r
+  | S n' => next (nextN n' r)
+  end.
+
+Notation "r + n" := (nextN n r).
+
+
+Lemma next_nextN r n : next (r + n) = next r + n.
+Proof.
+  generalize dependent r. induction n. reflexivity.
+  intros. simpl. rewrite IHn. reflexivity.
+Qed.
+
+Lemma lta_nextN r n : r < r + (S n).
+Proof.
+  induction n;simpl in *; auto.
+Qed.
+
+Lemma lta_next_eq (r r' : adr) : r < r' <-> exists n, r' = r + (S n).
+Proof.
+  split;intros.
+  - induction H.
+    + exists 0. reflexivity.
+    + destruct IHlta. exists (S x). simpl in *. subst. reflexivity.
+  - destruct H. subst. apply lta_nextN.
+Qed. 
+
+Lemma lea_lta r1 r2 r3 : r1 <= r2 -> r2 < r3 -> r1 < r3.
+Proof.
+  intros R1 R2. destruct R1. eauto. subst. assumption.
+Qed. 
+
+
+Lemma lta_lea r1 r2 r3 : r1 < r2 -> r2 <= r3 -> r1 < r3.
+Proof.
+  intros R1 R2. destruct R2. eauto. subst. assumption.
+Qed.
+
+Lemma lea_refl r : r <= r.
+Proof. unfold lea. auto. Qed.
+
+Lemma lta_to_lea r r' : r < r' -> r <= r'.
+Proof.
+  intro. unfold "<=". tauto.
+Qed.
+
+Lemma lea_sym r1 r2 r3 : r1 <= r2 -> r2 <= r3 -> r1 <= r3.
+Proof.
+  intros R1 R2.
+  destruct R1;subst;try assumption.
+  destruct R2; subst;try (left; assumption).
+  left. eauto.
+Qed. 
+
+Hint Resolve lta_lea lea_lta lea_sym lea_refl.
+
+(* Inductive eqr {T} (r : adr) : Mem T ->  Mem T -> Prop := *)
+(* | eqr_refl m : eqr r m m *)
+(* | eqr_set r' m v : r <= r' -> eqr r m (set r' v m) *)
+(* | eqr_trans m1 m2 m3 : eqr r m1 m2 -> eqr r m2 m3 -> eqr r m1 m3.  *)
+
+(* Notation "x =[ r ] y" := (eqr r x y) (at level 70). *)
+
+(* Hint Constructors eqr. *)
+
+
+
+(* Lemma eqr_set'  T r r' (m: Mem T) v : r <= r' -> set r' v m =[r] m. *)
+(* Proof. *)
+(*   intros l. apply eqr_set with (m0 := set r' v m) (v0 := get r' m) in l. *)
+(*   rewrite set_set in l. rewrite set_get in l. assumption. *)
+(* Qed.  *)
+
+
+(* Lemma eqr_sym T (x y : Mem T) r : x =[ r ] y -> y =[ r ] x. *)
+(* Proof. *)
+(*   intros R. induction R. *)
+(*   - constructor. *)
+(*   - apply eqr_set'; assumption. *)
+(*   - eapply eqr_trans;eassumption. *)
+(* Qed.  *)
+  
+
+(* Lemma eqr_lea T (x y : Mem T) r r' : x =[ r ] y -> r' <= r -> x =[ r' ] y. *)
+(* Proof. *)
+(*   intros R L. induction R; eauto. *)
+(* Qed. *)
+
+(* Lemma eqr_lta T (x y : Mem T) r r' : x =[ r ] y -> r' < r -> x =[ r' ] y. *)
+(* Proof. intros. eauto using eqr_lea, lta_to_lea. Qed. *)
+       
+
+(* Lemma set_eqr T n (s s' : Mem T) r r' : s =[r] s' -> r <= r' -> set r' n s =[r] s'. *)
+(* Proof. *)
+(*   intros H R. induction H. *)
+(*   - apply eqr_sym. auto. *)
+(*   - eapply eqr_trans. apply eqr_sym. apply eqr_set. *)
+(*     assumption. apply eqr_set. assumption. *)
+(*   - eapply eqr_trans. apply IHeqr1. assumption. *)
+(* Qed. *)
+
+
+(* (* Lemma set_get_eqr T r r' (s s' : Mem T) n : set r n s =[r'] s' -> r < r' -> get r s' = n. *) *)
+(* (* Proof. *) *)
+(* (*   intros R E. apply R in E. rewrite <- E. apply get_set. *) *)
+(* (* Qed. *) *)
+
+
+(* Definition rProp {T} (r: adr) (P : Mem T -> Prop) : Prop := forall s s', s =[r] s' -> (P s <-> P s'). *)
+
+
+(* Ltac rProp_log := unfold rProp; intros Pr Qr s s' E; *)
+(*   pose (Pr s s' E) as Pr'; pose (Qr s s' E) as Qr'; *)
+(*   rewrite Pr'; rewrite Qr'; tauto. *)
+
+(* Lemma rProp_conj r T (P Q : Mem T -> Prop) : rProp r P -> rProp r Q -> rProp r (fun s => P s /\ Q s). *)
+(* Proof. rProp_log. Qed.  *)
+
+(* Lemma rProp_disj r T (P Q : Mem T -> Prop) : rProp r P -> rProp r Q -> rProp r (fun s => P s \/ Q s). *)
+(* Proof. rProp_log. Qed. *)
+
+(* Lemma rProp_impl r T (P Q : Mem T -> Prop) : rProp r P -> rProp r Q -> rProp r (fun s => P s -> Q s). *)
+(* Proof. rProp_log. Qed. *)
+
+(* Lemma rProp_ex r T S (P : S -> Mem T -> Prop) : (forall a, rProp r (P a)) -> rProp r (fun s => exists a, P a s). *)
+(* Proof. *)
+(*   unfold rProp; intros Pr s s' E. *)
+(*   split; intros; destruct H; eexists. *)
+(*   rewrite <- Pr; eauto. *)
+(*   rewrite -> Pr; eauto. *)
+(* Qed. *)
+
+(* Lemma rProp_const T r P : rProp r (fun s : Mem T => P). *)
+(* Proof. *)
+(*   unfold rProp. tauto. *)
+(* Qed. *)
+
+(* Lemma eqr_get T (m m' : Mem T) r r' : *)
+(*   m =[r] m' -> r' < r -> get r' m = get r' m'. *)
+(* Proof. *)
+(*   intros R E. induction R. *)
+(*   - reflexivity. *)
+(*   - rewrite get_get. reflexivity. apply next_fresh. eauto. *)
+(*   - rewrite IHR1. rewrite <- IHR2. reflexivity. *)
+(* Qed.  *)
+
+(* Lemma rProp_get T r r' (v : T) : r' < r -> rProp r (fun s => get r' s = v). *)
+(* Proof. *)
+(*   unfold rProp. intros R s s' E. eapply eqr_get in E. rewrite E. tauto. assumption. *)
+(* Qed. *)
+
+(* Lemma rProp_eqr T r (s' : Mem T) : rProp r (fun s => s' =[r] s). *)
+(* Proof. *)
+(*   unfold rProp. intros s1 s2 E. split; eauto using eqr_sym, eqr_trans.  *)
+(* Qed. *)
+
+
+(* Lemma rProp_lea T r r' (P : Mem T -> Prop) : r < r' -> rProp r P -> rProp r' P. *)
+(* Proof. *)
+(*   unfold rProp. intros R Pr s s' E. eapply Pr. eauto using eqr_lta. *)
+(* Qed . *)
+
+(* Lemma rProp_ext T r (P : Mem T -> Prop) : rProp r P -> rProp r (fun s => P s). *)
+(* Proof. auto. Qed. *)
+
+(* Hint Resolve rProp_conj rProp_disj rProp_impl rProp_ex rProp_get rProp_lea rProp_ext rProp_const. *)
+
+(* Lemma rProp_set T (P : Mem T -> Prop) v s r r' : rProp r P -> r <= r' -> (P s <-> P (set r' v s)). *)
+(* Proof. *)
+(*   unfold rProp. intros Pr R. split;intro Ps; rewrite <- Pr; eauto using eqr_sym, eqr_set. *)
+(* Qed. *)
+
+(* Lemma rProp_set_r T (P : Mem T -> Prop) v s r: rProp r P -> P s -> P (set r v s). *)
+(* Proof. intros. rewrite <- rProp_set; eauto. Qed. *)
+
+(* Lemma rProp_set_l T (P : Mem T -> Prop) v s r : rProp r P -> P (set r v s) -> P s. *)
+(* Proof. intros. rewrite <- rProp_set in *; eauto. Qed. *)
+
+
+(* Lemma rProp_def T (P : Mem T -> Prop) r : *)
+(*   rProp r P <-> (forall m r' v, r <= r' -> (P m <-> P (set r' v m))). *)
+(* Proof. *)
+(*   split; intro. *)
+(*   - auto. *)
+(*   - intros m m' R. induction R. *)
+(*     * tauto. *)
+(*     * auto. *)
+(*     * rewrite IHR1. assumption. *)
+(* Qed . *)
+    
+
+End MemoryTheory.
