1stattempt/Arith.v
@@ -1,0 +1,75 @@
+(* Calculation of the simple arithmetic language. *)
+Require Import List.
+Require Import Tactics.
+
+
+Inductive Expr : Set :=  Val (n : nat) | Add (x y : Expr).
+
+Fixpoint eval (x: Expr) : nat :=
+  match x with
+    | Val n => n
+    | Add x1 x2 => eval x1 + eval x2
+  end.
+
+Inductive Instr : Set := .
+
+Definition Code := list Instr.
+
+Import ListNotations.
+
+
+Fixpoint comp (e : Expr) (c : Code) : Code :=
+  match e with
+    | Val n => Admit
+    | Add x y => Admit
+  end.
+
+Definition Stack : Set := list nat.
+
+Definition Conf : Set := prod Code  Stack.
+
+
+Hint Constructors VM.
+
+(* Boilerplate to import calculation tactics *)
+Module VM <: Machine.
+Definition Conf := Conf.
+Definition Rel := VM.
+End VM.
+Module VMCalc := Calculation VM.
+Import VMCalc.
+
+Ltac by_eval := eval_inv (eval).
+
+Theorem spec e P c :  { s, (comp e c, s) | P s} =|>
+                        { s n, (c , n :: s) | (e ⇓ n) /\ P s}.
+Proof.
+  intros.
+  generalize dependent c.
+  generalize dependent P.
+  induction e; intros.
+
+  begin
+    ({ s n', (c, n' :: s) | (Val n ⇓ n') /\ P s}).
+  = {by_eval}
+    ({ s, (c, n :: s) | P s}) .
+  <== {apply vm_push}
+    ({ s, (PUSH n :: c, s) | P s }) .
+  [].
+
+  begin
+  ({s n, (c, n :: s) | Add e1 e2 ⇓ n /\ P s }) .
+  = { by_eval }
+  ({s n m, (c, (n + m) :: s) | e1 ⇓ n /\ e2 ⇓ m /\ P s}) .
+  <== { apply vm_add }
+  ({ s n m, (ADD :: c, m :: n :: s) | e1 ⇓ n /\ e2 ⇓ m /\ P s}).
+  = { eauto }
+  ({s' m, (ADD :: c, m :: s') | e2 ⇓ m /\ (exists s n, e1 ⇓ n /\ s' = n :: s /\ P s)} ).
+  <|= { apply IHe2 }
+  ({s, (comp e2 (ADD :: c), s) | exists s' n, e1 ⇓ n /\ s = n :: s' /\ P s'}).
+  = { eauto }
+  ({s n, (comp e2 (ADD :: c),  n :: s) | e1 ⇓ n /\ P s }).
+  <|= { apply IHe1 }
+  ({s, (comp e1 (comp e2 (ADD :: c)),  s) | P s }).
+  [].
+Qed.
