1stattempt/SetOf.v
@@ -1,0 +1,176 @@
+Require Import List.
+Import ListNotations.
+
+  
+Fixpoint tuple (ts : list Type) : Type :=
+  match ts with
+    | []       => unit
+    | t :: ts' => (t * tuple ts')%type
+  end.
+
+
+Inductive SetCom (A : Type) : list Type -> Type :=
+| BaseSet : A -> Prop -> SetCom A nil
+| ExSet {t ts} : (t -> SetCom A ts) -> SetCom A (t :: ts).
+
+Arguments BaseSet {A} a p.
+Arguments ExSet {A} {t} {ts} p.
+
+Definition funtail {t ts A} (x : t) (f : forall (args : tuple (t :: ts)),  A args) 
+: forall (args : tuple ts), A (x, args) :=
+  fun xs => f (x, xs).
+
+
+Fixpoint mkSetCom {A ts} (C : tuple ts -> A) (P : tuple ts -> Prop) : SetCom A ts :=
+  match ts return (tuple ts -> A) -> (tuple ts -> Prop) -> SetCom A ts with
+    | nil => fun C P => BaseSet (C tt) (P tt)
+    | t :: ts' => fun C P => @ExSet A t ts'  (fun x => @mkSetCom A ts' (funtail x C) (funtail x P))
+  end C P.
+
+
+
+Fixpoint getConf {A ts} (S : SetCom A ts) : tuple ts -> A :=
+  match S with
+    | BaseSet C P => fun xs => C
+    | ExSet ex => fun xs =>  let (x, xs') := xs in  getConf (ex x) xs'
+  end.
+
+Fixpoint getProp {A ts} (S : SetCom A ts) : tuple ts -> Prop :=
+  match S with
+    | BaseSet C P => fun xs => P
+    | ExSet ex => fun xs => let (x, xs') := xs in getProp (ex x) xs'
+  end.
+
+Lemma getConf_sound A ts (C : tuple ts -> A) P x : getConf (mkSetCom C P) x = C x.
+Proof.
+  intros. induction ts; destruct x. reflexivity. simpl. apply (IHts (funtail a0 C)).
+Qed.
+
+
+Lemma getProp_sound A ts (C : tuple ts -> A) P x : getProp (mkSetCom C P) x = P x.
+Proof.
+  intros. induction ts;destruct x. reflexivity. simpl. apply (IHts _ (funtail a0 P)).
+Qed.
+
+Fixpoint  SetComElem  {A ts} (C : A) (S : SetCom A ts) : Prop :=
+  match S with
+      | BaseSet C' P => C' = C /\ P 
+      | ExSet e => exists x, SetComElem C (e x)
+  end.
+
+Lemma set_com_elem {A ts} (C : A) (S : SetCom A ts) : 
+  SetComElem C S <-> exists xs, getConf S xs = C /\ getProp S xs.
+Proof.
+  split; intros. 
+  * induction S.
+    - exists tt. assumption.
+
+    - simpl in H. destruct H. apply H0 in H.
+      decompose [ex and] H.  exists (x, x0). auto.
+  * induction S.
+    - decompose [ex and] H. simpl in *. tauto.
+    - decompose [ex and] H. simpl. destruct x.
+      exists t0. apply H0. exists t1. tauto.
+Qed.
+
+
+Inductive SetOf (A : Type) : Type :=
+  | Sing {ts} : SetCom A ts -> SetOf A
+  | Empty : SetOf A
+  | Union : SetOf A -> SetOf A -> SetOf A.
+
+Arguments Sing {A} {ts} s.
+Arguments Empty {A}.
+Arguments Union {A} s1 s2.
+
+
+Fixpoint ConfElem {A} (C : A) (S : SetOf A) : Prop :=
+  match S with
+    | Sing s => SetComElem C s
+    | Empty => False
+    | Union S1 S2 => ConfElem C S1 \/  ConfElem C S2
+  end.
+
+
+Notation "{| C | P |}" := (Sing (mkSetCom C P)) (at level 70, no associativity).
+Infix "∈" := ConfElem (at level 80, no associativity).
+Infix "∪" := Union (at level 76, left associativity).
+
+Definition Subset {A : Type} (S T : SetOf A) := (forall x, x ∈ S -> x ∈ T).
+
+
+Infix "⊆" := Subset (at level 80, no associativity).
+Infix "=<" := Subset (at level 80, no associativity).
+Notation "S == T" := (forall x, x ∈ S <-> x ∈ T) (at level 80, no associativity).
+
+
+Lemma mkSetComCompl' {A ts} (S : SetCom A ts) : {| getConf S | getProp S |} == Sing S.
+Proof.
+  simpl. unfold Subset. split; intros; induction S; auto; simpl in *; destruct H; eexists; apply H0; apply H.
+Qed.
+
+Lemma sing_set_elem {A ts} (C' : A) (C : tuple ts -> A) P :
+  C' ∈ {| C | P |} <-> exists xs, C xs = C' /\ P xs.
+Proof.
+  simpl. rewrite set_com_elem. split; intro H; decompose [ex and] H; eexists; 
+  rewrite getConf_sound in *; rewrite getProp_sound in *; split; eassumption.
+Qed.
+
+
+
+
+Notation "{ x .. y , C | P }" := (Sing (ExSet ( fun x =>  .. (ExSet (fun y => BaseSet C P)) ..  )))
+(at level 70, x binder, y binder, no associativity).
+
+
+Notation "{, C | P }" := (Sing (BaseSet C  P))
+(at level 70, no associativity).
+
+
+
+(* Lemma union_incll {A} (S T : SetOf A) : S ⊆ S ∪ T. *)
+(* Proof. simpl. auto. Qed. *)
+
+(* Lemma union_inclr {A} (S T : SetOf A) : T ⊆ S ∪ T. *)
+(* Proof. simpl. auto. Qed. *)
+
+(* Hint Resolve union_incll union_inclr. *)
+
+
+(* (* The above lemma cannot be used directly in a proof *)
+(* calculation. Therefore, we reformulat it using [getProp] and [getConf] *)
+(* instead of the [ {| C | P |} ] construction. *) *)
+
+(* Lemma union_sub_left {A} (S1 S2 T : SetOf A): S1 ⊆ S2 -> S1 ∪ T ⊆ S2 ∪ T . *)
+(* Proof. *)
+(*   intros. simpl in *. destruct H0; auto. *)
+(* Qed. *)
+
+(* Lemma union_eq_left {A} (S1 S2 T : SetOf A) : S1 == S2 -> S1 ∪ T == S2 ∪ T . *)
+(* Proof. *)
+(*   simpl in *; split;intros; destruct H0; solve [left; destruct H; auto| right; destruct H; auto]. *)
+(* Qed. *)
+
+(* Lemma union_sub_eq {A} (S1 S2: SetOf A) : S1 == S2 -> S1 ⊆ S2 . *)
+(* Proof. *)
+(*   intros. simpl in *. destruct H. auto. *)
+(* Qed. *)
+
+(* Lemma set_eq_ref {A} (S T: SetOf A) : S == T -> T == S. *)
+(* Proof. *)
+(*   intros. destruct H. split; auto. *)
+(* Qed. *)
+
+Lemma sub_union {A} (S1 S2 T1 T2 : SetOf A): S1 ⊆ S2 -> T1 ⊆ T2 -> S1 ∪ T2 ⊆ S2 ∪ T2 .
+Proof.
+  unfold Subset. intros. simpl in *. destruct H1; auto.
+Qed.
+
+Lemma sub_refl {A} (S : SetOf A): S ⊆ S .
+Proof. unfold Subset. auto. Qed.
+
+Lemma sub_trans {A} (S T U : SetOf A): S =< T -> T =< U -> S =< U .
+Proof. unfold Subset. auto. Qed.
+
+Lemma sub_eq {A} (S T : SetOf A): S == T -> S =< T .
+Proof. unfold Subset. intros.  apply (H x). auto. Qed.
